more cleanup

concurrency/scache/AtomicIndexLookup.i.dfy
@@ -1,7 +1,7 @@
 include "../framework/Atomic.s.dfy"
 include "../../lib/Lang/NativeTypes.s.dfy"
-include "../../lib/Base/LinearOption.i.dfy"
-include "CacheResources.i.dfy"
+include "../framework/GlinearOption.i.dfy"
+include "cache/CacheResources.i.dfy"
 include "Constants.i.dfy"
 include "../framework/Ptrs.s.dfy"
 
@@ -12,105 +12,95 @@ module AtomicIndexLookupImpl {
   import opened Constants
   import opened CacheResources
   import opened Options
-  import opened LinearOption
+  import opened GlinearOption
+  import opened CacheStatusType
 
-  type AtomicIndexLookup = Atomic<uint64, CacheResources.R>
+  type AtomicIndexLookup = Atomic<uint64, CacheResources.DiskPageMap>
 
   const NOT_MAPPED : uint64 := 0xffff_ffff_ffff_ffff;
 
-  predicate state_inv(v: uint64, g: CacheResources.R, disk_idx: nat)
+  predicate state_inv(v: uint64, g: CacheResources.DiskPageMap, disk_idx: nat)
   {
     && (0 <= v as int < CACHE_SIZE || v == NOT_MAPPED)
     && g == CacheResources.DiskPageMap(disk_idx,
-        (if v == NOT_MAPPED then None else Some(v)))
+        (if v == NOT_MAPPED then None else Some(v as nat)))
   }
 
-  predicate atomic_index_lookup_inv(a: AtomicIndexLookup, disk_idx: int)
+  predicate atomic_index_lookup_inv(a: AtomicIndexLookup, disk_idx: nat)
   {
     forall v, g :: atomic_inv(a, v, g) <==> state_inv(v, g, disk_idx)
   }
 
   method atomic_index_lookup_read(
       a: AtomicIndexLookup,
-      disk_idx: int)
+      disk_idx: nat)
   returns (cache_idx: uint64)
   requires atomic_index_lookup_inv(a, disk_idx)
   ensures 0 <= cache_idx as int < CACHE_SIZE || cache_idx == NOT_MAPPED
 
   method atomic_index_lookup_clear_mapping(
       a: AtomicIndexLookup,
-      disk_idx: int,
-      linear cache_entry: CacheResources.R,
-      linear status: CacheResources.R
+      disk_idx: nat,
+      glinear cache_entry: CacheResources.CacheEntry,
+      glinear status: CacheResources.CacheStatus
   )
   returns (
-      linear cache_entry': CacheResources.R,
-      linear status': CacheResources.R
+      glinear cache_entry': CacheResources.CacheEmpty
   )
   requires atomic_index_lookup_inv(a, disk_idx)
   requires status.CacheStatus?
-  requires status.status == CacheResources.Clean
+  requires status.status == Clean
   requires cache_entry.CacheEntry?
   requires cache_entry.cache_idx == status.cache_idx
-  ensures status' == status.(status := CacheResources.Empty)
-  ensures cache_entry' == cache_entry
+  ensures cache_entry' == CacheEmpty(cache_entry.cache_idx)
 
   method atomic_index_lookup_add_mapping(
       a: AtomicIndexLookup,
       disk_idx: uint64,
       cache_idx: uint64,
-      linear cache_entry: CacheResources.R,
-      linear status: CacheResources.R)
+      glinear cache_empty: CacheResources.CacheEmpty)
   returns (
     success: bool,
-    linear cache_entry': CacheResources.R,
-    linear status': CacheResources.R,
-    linear read_ticket: lOption<DiskReadTicket>
+    glinear cache_empty': glOption<CacheResources.CacheEmpty>,
+    glinear cache_reading': glOption<CacheResources.CacheReading>,
+    glinear read_ticket: glOption<CacheResources.DiskReadTicket>
   )
   requires atomic_index_lookup_inv(a, disk_idx as int)
-  requires cache_entry.CacheEntry?
-  requires cache_entry.cache_idx == cache_idx as int
-  requires status == CacheStatus(cache_idx as int, Empty)
+  requires cache_empty.cache_idx == cache_idx as int
   requires 0 <= cache_idx as int < CACHE_SIZE
-  ensures !success ==> cache_entry' == cache_entry
-  ensures success ==> cache_entry' ==
-      cache_entry.(disk_idx := disk_idx as int)
-  ensures !success ==> status' == status
-  ensures success ==> status' == CacheStatus(cache_idx as int, Reading)
-  ensures success ==>
-      && read_ticket == lSome(DiskReadTicket(disk_idx))
-  ensures !success ==> read_ticket == lNone
-  {
-    var did_set := compare_and_set(a, NOT_MAPPED, cache_idx);
+  ensures !success ==> cache_empty' == glSome(cache_empty)
+  ensures !success ==> cache_reading' == glNone
+  ensures !success ==> read_ticket == glNone
 
-    ///// Begin jank
-    ///// Setup:
-    var v1 := NOT_MAPPED;
-    var v2 := cache_idx;
-    var old_v: uint64;
-    var new_v: uint64;
-    linear var old_g: CacheResources.R := unsafe_obtain();
-    assume old_v == v1 ==> new_v == v2 && did_set;
-    assume old_v != v1 ==> new_v == old_v && !did_set;
-    assume atomic_inv(a, old_v, old_g);
-    linear var new_g;
-    ///// Transfer:
-    if did_set {
-      linear var ticket;
-      status', cache_entry', new_g, ticket :=
-        initiate_page_in(cache_idx as int, disk_idx, status, cache_entry, old_g);
-      read_ticket := lSome(ticket);
-    } else {
-      cache_entry' := cache_entry;
-      status' := status;
-      read_ticket := lNone;
-      new_g := old_g;
+  ensures success ==> cache_empty' == glNone
+  ensures success ==> cache_reading' ==
+    glSome(CacheReading(cache_idx as nat, disk_idx as nat))
+  ensures success ==>
+      && read_ticket == glSome(DiskReadTicket(disk_idx as int))
+  {
+    atomic_block var did_set :=
+      execute_atomic_compare_and_set_strong(a, NOT_MAPPED, cache_idx)
+    {
+      ghost_acquire old_g;
+      glinear var new_g;
+
+      if did_set {
+        glinear var ticket, cr;
+        cr, new_g, ticket := CacheResources.initiate_page_in(
+            cache_idx as int, disk_idx as int, cache_empty, old_g);
+        read_ticket := glSome(ticket);
+        cache_reading' := glSome(cr);
+        cache_empty' := glNone;
+      } else {
+        cache_empty' := glSome(cache_empty);
+        cache_reading' := glNone;
+        read_ticket := glNone;
+        new_g := old_g;
+      }
+      assert state_inv(new_value, new_g, disk_idx as int);
+
+      ghost_release new_g;
     }
-    assert state_inv(new_v, new_g, disk_idx as int);
-    ///// Teardown:
-    assert atomic_inv(a, new_v, new_g);
-    unsafe_dispose(new_g);
-    ///// End jank
 
     success := did_set;
   }
